STLCWA almost finished.

STLCWA.v
@@ -1,8 +1,11 @@
 
 Require Import SfLib.
 
+Require Import Coq.Relations.Relation_Definitions.
+
 
 Module STLCARITH.
+
 
 Inductive ty : Type :=
     | TArrow : ty -> ty -> ty
@@ -37,7 +40,7 @@ Fixpoint byContext (ctx : Context) (i : id) : option ty :=
 
 Reserved Notation "Gamma '|=' t '\in' T" (at level 40).            
 
-Inductive has_type : Context -> tm -> ty -> Type :=
+Inductive has_type : Context -> tm -> ty -> Prop :=
     | tyVar : 
         forall G i T,
             byContext G i = Some T ->
@@ -84,7 +87,7 @@ Fixpoint subst (i : id) (t org : tm) : tm :=
     match org with
         | tvar j => if(eq_id_dec i j) then t else org
         | tapp a b => tapp ([i := t] a) ([i := t] b)
-        | tabs x T y => tabs x T (if (eq_id_dec i x) then y else ([i := t] y))
+        | tabs x T y => tabs x T (if (eq_id_dec x i) then y else ([i := t] y))
         | tsucc x => tsucc ([i := t] x)
         | tpred y => tpred ([i := t] y)
         | tmult x y => tmult ([i := t] x) ([i := t] y)
@@ -307,6 +310,456 @@ Theorem progress :
     exists (tif0 x t1 t2); eauto.
 Qed.
 
+Theorem preservation :
+    forall t t' T,
+        empty |= t \in T ->
+        step t t' ->
+        empty |= t' \in T.
+
+    intro. elim t; intros.
+    inversion H0.
+    
+    inversion H1; inversion H2; subst; eauto.
+
+    Abort.
+
+Lemma app_preserv:
+    forall t x y T G U,
+        U |= tabs x T t \in TArrow T G ->
+        empty |= y \in T ->
+        U |= [x := y] t \in G.
+    intro t. elim t; intros.
+    inversion H; subst. unfold subst.
+    inversion H3; subst. unfold byContext in *. 
+    destruct (eq_id_dec i x); subst. inversion H4; subst.
+    rewrite eq_id_dec_id.
+
+    Abort.
+
+
+(*
+Theorem update_shadow:
+    forall U i x y,
+    update i x (update i y U) =-= update i x U.
+
+    unfold context_equivalence.
+    intro. induction U; intros.
+    unfold byContext in *.
+    destruct (eq_id_dec i0 i); subst; auto.
+
+    unfold byContext in *.
+    destruct (eq_id_dec i1 i0); subst; auto.
+
+Qed.
+
+Theorem update_permute:
+    forall U i j x y,
+    i <> j ->
+    update i x (update j y U) =-= update j y (update i x U).
+
+    intro. 
+    
+    induction U; intros.
+    unfold context_equivalence. intros.
+    unfold byContext in *. destruct (eq_id_dec i0 i); destruct (eq_id_dec i0 j); subst; eauto.
+    destruct (H eq_refl).
+
+    destruct (eq_id_dec i j); subst.
+    Abort.
+
+Print relation.
+Print equiv.
+
+Theorem equiv_ctx_eq:
+    equiv context_equivalence.
+*)
+
+Definition context_equivalence : relation Context :=
+    fun (x y : Context) => forall i, byContext x i = byContext y i.
+
+Notation "x '=-=' y" := (context_equivalence x y) (at level 40).
+
+
+Print reflexive.
+Print equiv.
+
+Theorem equiv_ctx_eq:
+    equiv _ context_equivalence.
+
+    unfold equiv; split.
+    unfold reflexive; intros. intro. auto.
+    split. unfold transitive.
+    intros x y. generalize dependent x.
+    elim y. intros.
+    unfold context_equivalence in *.
+    intros; eauto. 
+    rewrite H. rewrite H0. auto.
+
+
+(*
+    unfold context_equivalence in *.
+    
+    intros. cbn in *.
+    destruct (eq_id_dec i0 i); subst. 
+    pose (H0 i); pose (H1 i). repeat rewrite eq_id_dec_id in *.
+    rewrite e; auto.
+
+    assert (forall i, byContext x i = byContext c i).
+    intros.
+    destruct (eq_id_dec i0 i). pose (H0 i0). 
+*)
+    intros i t c h x. generalize dependent i;
+    generalize dependent t; generalize dependent h.
+    induction x. intros. unfold context_equivalence in *.
+    pose (H i). inversion e. rewrite eq_id_dec_id in *. inversion H2.
+    intros. 
+    Abort.
+
+Theorem refl_ctxeq:
+    reflexive _ context_equivalence.
+    unfold reflexive; unfold context_equivalence. auto.
+Qed.
+
+Theorem symm_ctxeq:
+    symmetric _ context_equivalence.
+    unfold symmetric; unfold context_equivalence. auto.
+Qed.
+
+Theorem update_shadow:
+    forall i x y U V,
+        U =-= V ->
+        update i x (update i y U) =-= update i x V.
+        
+    unfold context_equivalence. intros.
+    cbn. destruct (eq_id_dec i0 i); auto.
+
+Qed.
+
+Theorem update_permute :
+    forall i j x y U V,
+        i <> j ->
+        U =-= V ->
+        update i x (update j y U) =-= update j y (update i x U).
+
+    unfold context_equivalence. 
+    intros. cbn. destruct (eq_id_dec i0 i); destruct (eq_id_dec i0 j); auto; subst.
+    destruct (H eq_refl).
+Qed.
+
+Theorem update_inc:
+    forall i x U V,
+        U =-= V ->
+        update i x U =-= update i x V.
+
+    unfold context_equivalence.
+    intros. cbn. destruct (eq_id_dec i0 i); subst; auto.
+Qed.
+
+Inductive occurs_free : id -> tm -> Prop :=
+    | occurs_free_var :
+        forall i,
+            occurs_free i (tvar i)
+    | occurs_free_abs :
+        forall i j x T,
+            occurs_free i x ->
+            i <> j ->
+            occurs_free i (tabs j T x)
+    | occurs_free_app1 :
+        forall i x y,
+            occurs_free i x ->
+            occurs_free i (tapp x y)
+    | occurs_free_app2 :
+        forall i x y,
+            occurs_free i y ->
+            occurs_free i (tapp x y)
+    | occurs_free_succ :
+        forall i x,
+            occurs_free i x ->
+            occurs_free i (tsucc x)
+    | occurs_free_pred :
+        forall i x,
+            occurs_free i x ->
+            occurs_free i (tpred x)
+    | occurs_free_mult1 :
+        forall i x y,
+            occurs_free i x ->
+            occurs_free i (tmult x y)
+    | occurs_free_mult2 :
+        forall i x y,
+            occurs_free i y ->
+            occurs_free i (tmult x y)
+    | occurs_free_if0 :
+        forall i t t0 t1,
+            occurs_free i t ->
+            occurs_free i (tif0 t t0 t1)
+    | occurs_free_if1 :
+        forall i t t0 t1,
+            occurs_free i t0 ->
+            occurs_free i (tif0 t t0 t1)
+    | occurs_free_if2 :
+        forall i t t0 t1,
+            occurs_free i t1 ->
+            occurs_free i (tif0 t t0 t1).
+
+    Hint Constructors occurs_free.
+Theorem occurs_dec:
+    forall i x,
+    {occurs_free i x} + {~occurs_free i x}.
+
+    intros i x. generalize dependent i.
+    induction x; eauto.
+    intros. 
+    destruct (eq_id_dec i0 i); subst. 
+    left; eauto.
+    right; intros H; inversion H; subst. destruct (n eq_refl).
+
+    intros. destruct (IHx1 i). left; eauto.
+    destruct (IHx2 i). left; eauto.
+    right; intro. inversion H; subst; eauto.
+
+    intro. destruct (IHx i0). destruct (eq_id_dec i0 i); subst.
+    right; intro HH; inversion HH; subst. destruct (H4 eq_refl).
+    left; eauto.
+
+    right; intro HH; inversion HH; subst; eauto.
+
+    intros; right; intro HH; inversion HH.
+
+    intros i; destruct (IHx i). left; eauto. right; intro HH; inversion HH; subst; eauto.
+
+    intros i; destruct (IHx i). left; eauto. right; intro HH; inversion HH; subst; eauto.
+    
+    intros i; destruct (IHx1 i).
+    left; eauto. destruct (IHx2 i). left; eauto.
+    right; intro HH; inversion HH; subst; eauto.
+
+    intros i; destruct (IHx1 i).
+    left; eauto. destruct (IHx2 i). left; eauto.
+    destruct (IHx3 i). left; eauto.
+    right; intro HH; inversion HH; subst; eauto.
+Qed.
+
+Definition closed (x : tm) :=
+    forall i, ~ occurs_free i x.
+
+Theorem ctx_swap:
+    forall x U V T ,
+        U |= x \in T ->
+        U =-= V ->
+        V |= x \in T.
+
+    intros x U V T h.
+    generalize dependent V.
+    induction h; unfold context_equivalence; intros; eauto.
+    eapply tyVar. rewrite <- H0. auto.
+
+    eapply tyAbs. 
+    pose (update_inc).
+    pose (update_inc i G _ _ H).
+    eauto.
+Qed.
+
+Theorem non_occurs_free_ctx_rm:
+    forall v i x U T,
+    update i x U |= v \in T ->
+    (~occurs_free i v) ->
+    U |= v \in T.
+
+    intros v i x U T h.
+    remember (update i x U) as u.
+    generalize Hequ.
+    induction h; subst; eauto.
+    intros. cbn in H. 
+    destruct (eq_id_dec i0 i); subst. destruct (H0 (occurs_free_var i)).
+    eauto.
+
+    intros. 
+    pose (contrapositive _ _ (occurs_dec _ _) (occurs_free_app1 i a b)).
+    pose (contrapositive _ _ (occurs_dec _ _) (occurs_free_app2 i a b)).
+
+    pose (IHh2 eq_refl eq_refl).
+    pose (IHh1 eq_refl eq_refl).
+    eapply tyApp; eauto.
+
+    intros. destruct (occurs_dec i x0). 
+    destruct (eq_id_dec i i0); subst.
+    
+    pose (update_shadow i0 G x U U (refl_ctxeq _ )).
+    pose (ctx_swap _ _ _ _ h c).
+    eauto.
+
+    assert (occurs_free i (tabs i0 G x0)) as HH; eauto.
+    destruct (H HH).
+
+    eauto.
+    Abort.
+
+
+Theorem non_occurs_free_ctx_rm:
+    forall v i x U T,
+    update i x U |= v \in T ->
+    (~occurs_free i v) ->
+    U |= v \in T.
+
+    intro v; induction v; eauto.
+    intros. inversion H; subst.
+    cbn in H3. destruct (eq_id_dec i i0); subst.
+    destruct (H0 (occurs_free_var i0)).
+    eauto.
+
+    intros. 
+    pose (contrapositive _ _ (occurs_dec _ _) (occurs_free_app1 i v1 v2)).
+    pose (contrapositive _ _ (occurs_dec _ _) (occurs_free_app2 i v1 v2)).
+    inversion H; subst. eapply tyApp; eauto.
+
+    intros. inversion H; subst.
+    destruct (occurs_dec i0 v);
+    destruct (eq_id_dec i0 i); subst. inversion H; subst.
+    
+    pose (update_shadow i t x U U (refl_ctxeq _ )).
+    pose (ctx_swap _ _ _ _ H6 c).
+    eauto.
+
+    assert (occurs_free i0 (tabs i t v)) as HH; eauto.
+    destruct (H0 HH).
+
+    inversion H; subst. 
+    pose (update_shadow i t x U U (refl_ctxeq _ )).
+    pose (ctx_swap _ _ _ _ H6 c).
+    eauto.
+    pose (update_permute i0 i x t U U n0 (refl_ctxeq _)).
+    Print symm_ctxeq.
+    pose (symm_ctxeq _ _ c).
+    pose (ctx_swap _ _ _ _ H6 c0).
+    eauto.
+
+    intros. inversion H; subst. eauto.
+
+    intros. inversion H; subst.
+    Print occurs_free_succ. 
+    pose (contrapositive _ _ (occurs_dec _ _) (occurs_free_succ i v)).
+    eauto.
+
+    intros. inversion H; subst.
+    pose (contrapositive _ _ (occurs_dec _ _) (occurs_free_pred i v)).
+    eauto.
+
+    intros. inversion H; subst.
+    pose (contrapositive _ _ (occurs_dec _ _) (occurs_free_mult1 i v1 v2)).
+    pose (contrapositive _ _ (occurs_dec _ _) (occurs_free_mult2 i v1 v2)).
+    eapply tyMult; eauto.
+
+    intros.
+     inversion H; subst.
+     pose (contrapositive _ _ (occurs_dec _ _) (occurs_free_if0 i v1 v2 v3)).
+     pose (contrapositive _ _ (occurs_dec _ _) (occurs_free_if1 i v1 v2 v3)).
+     pose (contrapositive _ _ (occurs_dec _ _) (occurs_free_if2 i v1 v2 v3)).
+     eapply tyIf; eauto.
+
+Qed.
+
+   
+Lemma occurs_free_is_in_ctx:
+forall i x U T,
+    U |= x \in T ->
+    occurs_free i x ->
+    (exists K, byContext U i = Some K).
+
+intros i x U T h0 h.
+generalize dependent U.
+generalize dependent T.
+induction h; intros; eauto; try (inversion h0; subst; eauto).
+
+inversion h0; subst. 
+destruct (IHh _ _ H5).
+cbn in H0. destruct (eq_id_dec i j); subst; eauto.
+destruct (H eq_refl).
+Qed.
+
+
+
+Theorem empty_means_closed:
+    forall t T,
+        empty |= t \in T ->
+        closed t.
+
+    unfold closed.
+    intros t.
+    induction t; intros; intro.
+    inversion H; subst. inversion H3.
+
+    inversion H; subst. inversion H0; subst. 
+    destruct ((IHt1 _ H4 i) H3).
+    destruct ((IHt2 _ H6 i) H3).
+
+ 
+
+    inversion H; subst; inversion H0; subst.
+    destruct (occurs_free_is_in_ctx _ _ _ _ H H0).
+    inversion H1.
+
+    inversion H0. 
+
+    inversion H; inversion H0; subst; eauto.
+    eapply IHt. apply H3. apply H7.
+
+    inversion H; inversion H0; subst; eapply IHt. apply H3. apply H7.
+    inversion H; inversion H0; subst. eapply IHt1; eauto. eapply IHt2; eauto.
+    inversion H; inversion H0; subst. eapply IHt1; eauto. eapply IHt2; eauto. eapply IHt3; eauto.
+
+Qed.
+
+
+    
+
+
+
+
+
+
+
+     
+    
+
+
+
+    
+
+
+
+
+
+
+
+
+    
+
+
+    
+
+
+    
+
+
+
+
+
+
+
+
+
+
+
+
+
+
+
+
+
+
+
+
+    
 
 
 
